proof/invariant-abstract/RISCV64/ArchInvariants_AI.thy
@@ -31,7 +31,7 @@ abbreviation
   "vs_lookup s \<equiv> \<lambda>level asid vref. vs_lookup_table level asid vref s"
 
 locale_abbrev
-  "atyps_of \<equiv> \<lambda>s. aobjs_of s ||> aa_type"
+  "atyps_of \<equiv> \<lambda>s. aobjs_of False s ||> aa_type"
 
 definition arch_tcb_to_iarch_tcb :: "arch_tcb \<Rightarrow> iarch_tcb" where
   "arch_tcb_to_iarch_tcb arch_tcb \<equiv> Void ()"
@@ -290,7 +290,7 @@ primrec valid_vspace_obj :: "vm_level \<Rightarrow> arch_kernel_obj \<Rightarrow
 | "valid_vspace_obj _ (DataPage _ _) = \<top>" (* already covered by valid_pte *)
 
 definition valid_vso_at :: "vm_level \<Rightarrow> obj_ref \<Rightarrow> 'z::state_ext state \<Rightarrow> bool" where
-  "valid_vso_at level p \<equiv> \<lambda>s. \<exists>ao. aobjs_of s p = Some ao \<and> valid_vspace_obj level ao s"
+  "valid_vso_at level p \<equiv> \<lambda>s. \<exists>ao. aobjs_of False s p = Some ao \<and> valid_vspace_obj level ao s"
 
 definition wellformed_pte :: "pte \<Rightarrow> bool" where
   "wellformed_pte pte \<equiv> is_PagePTE pte \<longrightarrow> pte_rights pte \<in> valid_vm_rights"
@@ -307,18 +307,18 @@ definition wellformed_vspace_obj :: "arch_kernel_obj \<Rightarrow> bool" where
 
 lemmas wellformed_aobj_simps[simp] = wellformed_aobj_def[split_simps arch_kernel_obj.split]
 
-definition has_kernel_mappings :: "pt \<Rightarrow> 'z::state_ext state \<Rightarrow> bool" where
-  "has_kernel_mappings pt \<equiv> \<lambda>s.
-     \<forall>pt'. pts_of s (global_pt s) = Some pt' \<longrightarrow>
+definition has_kernel_mappings :: "bool \<Rightarrow> pt \<Rightarrow> 'z::state_ext state \<Rightarrow> bool" where
+  "has_kernel_mappings ta_f pt \<equiv> \<lambda>s.
+     \<forall>pt'. pts_of False s (global_pt s) = Some pt' \<longrightarrow>
            (\<forall>i \<in> kernel_mapping_slots. pt i = pt' i)"
 
 (* To find the top-level page tables, we need to start with ASIDs *)
-definition equal_kernel_mappings :: "'z::state_ext state \<Rightarrow> bool" where
-  "equal_kernel_mappings \<equiv> \<lambda>s.
+definition equal_kernel_mappings :: "bool \<Rightarrow> 'z::state_ext state \<Rightarrow> bool" where
+  "equal_kernel_mappings ta_f \<equiv> \<lambda>s.
      \<forall>asid pt_ptr pt.
-       vspace_for_asid asid s = Some pt_ptr
-      \<longrightarrow> pts_of s pt_ptr = Some pt
-      \<longrightarrow> has_kernel_mappings pt s"
+       vspace_for_asid ta_f asid s = Some pt_ptr
+      \<longrightarrow> pts_of False s pt_ptr = Some pt
+      \<longrightarrow> has_kernel_mappings ta_f pt s"
 
 definition pte_ref :: "pte \<Rightarrow> obj_ref option" where
   "pte_ref pte \<equiv> case pte of
@@ -331,9 +331,9 @@ lemmas pte_ref_simps[simp] = pte_ref_def[split_simps pte.split]
 definition valid_vspace_objs :: "'z::state_ext state \<Rightarrow> bool" where
   "valid_vspace_objs \<equiv> \<lambda>s.
      \<forall>bot_level asid vref level p ao.
-       vs_lookup_table bot_level asid vref s = Some (level, p)
+       vs_lookup_table False bot_level asid vref s = Some (level, p)
        \<longrightarrow> vref \<in> user_region
-       \<longrightarrow> aobjs_of s p = Some ao
+       \<longrightarrow> aobjs_of False s p = Some ao
        \<longrightarrow> valid_vspace_obj level ao s"
 
 (* Mask out the bits that will not be used for lookups down to specified level *)
@@ -346,7 +346,7 @@ definition asid_for_level :: "asid \<Rightarrow> vm_level \<Rightarrow> asid" wh
      if level = asid_pool_level then asid && ~~mask asid_low_bits else asid"
 
 locale_abbrev pte_refs_of :: "'z::state_ext state \<Rightarrow> obj_ref \<Rightarrow> obj_ref option" where
-  "pte_refs_of \<equiv> \<lambda>s. ptes_of s |> pte_ref"
+  "pte_refs_of \<equiv> \<lambda>s. ptes_of False s |> pte_ref"
 
 (* vs_lookup_slot locates a slot at a given level,
    vs_lookup_target returns the object reference in that slot. *)
@@ -354,9 +354,9 @@ definition vs_lookup_target ::
   "vm_level \<Rightarrow> asid \<Rightarrow> vspace_ref \<Rightarrow> 'z::state_ext state \<Rightarrow> (vm_level \<times> obj_ref) option"
   where
   "vs_lookup_target bot_level asid vref \<equiv> do {
-     (level, slot) \<leftarrow> vs_lookup_slot bot_level asid vref;
+     (level, slot) \<leftarrow> vs_lookup_slot False bot_level asid vref;
      ptr \<leftarrow> if level = asid_pool_level
-            then vspace_for_pool slot asid \<circ> asid_pools_of
+            then vspace_for_pool slot asid \<circ> asid_pools_of False
             else swp pte_refs_of slot;
      oreturn (level, ptr)
   }"
@@ -433,7 +433,7 @@ definition valid_table_caps_2 :: "(cslot_ptr \<rightharpoonup> cap) \<Rightarrow
          pts r = Some empty_pt"
 
 locale_abbrev valid_table_caps :: "'z::state_ext state \<Rightarrow> bool" where
-  "valid_table_caps \<equiv> \<lambda>s. valid_table_caps_2 (caps_of_state s) (pts_of s)"
+  "valid_table_caps \<equiv> \<lambda>s. valid_table_caps_2 (caps_of_state s) (pts_of False s)"
 
 lemmas valid_table_caps_def = valid_table_caps_2_def
 
@@ -515,7 +515,7 @@ definition valid_global_tables_2 :: "(RISCV64_A.vm_level \<Rightarrow> obj_ref s
 
 locale_abbrev valid_global_tables :: "'z::state_ext state \<Rightarrow> bool" where
   "valid_global_tables \<equiv>
-    \<lambda>s. valid_global_tables_2 (riscv_global_pts (arch_state s)) (pts_of s)"
+    \<lambda>s. valid_global_tables_2 (riscv_global_pts (arch_state s)) (pts_of False s)"
 
 lemmas valid_global_tables_def = valid_global_tables_2_def
 
@@ -530,7 +530,7 @@ definition valid_asid_table_2 :: "(asid_high_index \<rightharpoonup> obj_ref) \<
   "valid_asid_table_2 table pools \<equiv> ran table \<subseteq> dom pools \<and> inj_on table (dom table)"
 
 locale_abbrev valid_asid_table :: "'z::state_ext state \<Rightarrow> bool" where
-  "valid_asid_table \<equiv> \<lambda>s. valid_asid_table_2 (asid_table s) (asid_pools_of s)"
+  "valid_asid_table \<equiv> \<lambda>s. valid_asid_table_2 (asid_table s) (asid_pools_of False s)"
 
 lemmas valid_asid_table_def = valid_asid_table_2_def
 
@@ -551,8 +551,8 @@ definition valid_global_vspace_mappings :: "'z::state_ext state \<Rightarrow> bo
   "valid_global_vspace_mappings \<equiv> \<lambda>s.
      let root = global_pt s in
        is_aligned root pt_bits \<and>
-       (\<forall>vref \<in> kernel_window s. translate_address root vref (ptes_of s) = Some (addrFromPPtr vref)) \<and>
-       (\<forall>vref \<in> kernel_elf_window s. translate_address root vref (ptes_of s) = Some (addrFromKPPtr vref))"
+       (\<forall>vref \<in> kernel_window s. translate_address root vref (ptes_of False s) = Some (addrFromPPtr vref)) \<and>
+       (\<forall>vref \<in> kernel_elf_window s. translate_address root vref (ptes_of False s) = Some (addrFromKPPtr vref))"
 
 locale_abbrev obj_addrs :: "kernel_object \<Rightarrow> obj_ref \<Rightarrow> obj_ref set" where
   "obj_addrs ko p \<equiv> {p .. p + 2 ^ obj_bits ko - 1}"
@@ -562,7 +562,7 @@ definition pspace_in_kernel_window :: "'z::state_ext state \<Rightarrow> bool" w
   "pspace_in_kernel_window \<equiv> \<lambda>s. \<forall>p ko. kheap s p = Some ko \<longrightarrow> obj_addrs ko p \<subseteq> kernel_window s"
 
 definition vspace_at_asid :: "asid \<Rightarrow> obj_ref \<Rightarrow> 'z::state_ext state \<Rightarrow> bool" where
-  "vspace_at_asid asid pt \<equiv> \<lambda>s. vspace_for_asid asid s = Some pt"
+  "vspace_at_asid asid pt \<equiv> \<lambda>s. vspace_for_asid False asid s = Some pt"
 
 definition valid_uses_2 :: "(obj_ref \<Rightarrow> riscvvspace_region_use) \<Rightarrow> bool" where
   "valid_uses_2 uses \<equiv>
@@ -869,7 +869,7 @@ section \<open>Basic Properties\<close>
 
 lemma valid_table_caps_pdD:
   "\<lbrakk> caps_of_state s p = Some (ArchObjectCap (PageTableCap pt None)); valid_table_caps s \<rbrakk>
-  \<Longrightarrow> pts_of s pt = Some empty_pt"
+  \<Longrightarrow> pts_of False s pt = Some empty_pt"
   by (auto simp add: valid_table_caps_def simp del: split_paired_Ex)
 
 lemma addrFromPPtr_ptrFromPAddr_id[simp]:
@@ -1021,17 +1021,17 @@ lemma pt_of_Some[iff]:
   by (simp add: pt_of_def split: arch_kernel_obj.splits)
 
 lemma aobjs_of_Some:
-  "(aobjs_of s p = Some ao) = (f_kheap s p = Some (ArchObj ao))"
+  "(aobjs_of ta_f s p = Some ao) = (f_kheap ta_f s p = Some (ArchObj ao))"
   by (simp add: in_omonad)
 
 lemma pts_of_Some:
-  "(pts_of s p = Some pt) = (aobjs_of s p = Some (PageTable pt))"
+  "(pts_of ta_f s p = Some pt) = (aobjs_of ta_f s p = Some (PageTable pt))"
   by (simp add: in_omonad)
 
 lemma ptes_of_Some:
-  "(ptes_of s p = Some pte) =
+  "(ptes_of ta_f s p = Some pte) =
    ((\<exists>pt. is_aligned p pte_bits \<and>
-          pts_of s (p && ~~ mask pt_bits) = Some pt \<and>
+          pts_of ta_f s (p && ~~ mask pt_bits) = Some pt \<and>
           pt (ucast (p && mask pt_bits >> pte_bits)) = pte))"
   by (auto simp: pte_of_def in_omonad)
 
@@ -1045,32 +1045,32 @@ lemma aa_typeE[elim!]:
   by (cases ao; clarsimp split: if_split_asm)+
 
 lemma atyp_at_eq_kheap_obj:
-  "typ_at (AArch AASIDPool) p s \<longleftrightarrow> (\<exists>f. f_kheap s p = Some (ArchObj (ASIDPool f)))"
-  "typ_at (AArch APageTable) p s \<longleftrightarrow> (\<exists>pt. f_kheap s p = Some (ArchObj (PageTable pt)))"
-  "typ_at (AArch (AUserData sz)) p s \<longleftrightarrow> (f_kheap s p = Some (ArchObj (DataPage False sz)))"
-  "typ_at (AArch (ADeviceData sz)) p s \<longleftrightarrow> (f_kheap s p = Some (ArchObj (DataPage True sz)))"
-  by (auto simp: obj_at_def)
+  "typ_at (AArch AASIDPool) p s \<longleftrightarrow> (\<exists>f. kheap s p = Some (ArchObj (ASIDPool f)))"
+  "typ_at (AArch APageTable) p s \<longleftrightarrow> (\<exists>pt. kheap s p = Some (ArchObj (PageTable pt)))"
+  "typ_at (AArch (AUserData sz)) p s \<longleftrightarrow> (kheap s p = Some (ArchObj (DataPage False sz)))"
+  "typ_at (AArch (ADeviceData sz)) p s \<longleftrightarrow> (kheap s p = Some (ArchObj (DataPage True sz)))"
+  by (auto simp: obj_at_def obind_def split:option.splits)
 
 lemma asid_pools_at_eq:
-  "asid_pool_at p s \<longleftrightarrow> asid_pools_of s p \<noteq> None"
-  by (auto simp: obj_at_def in_opt_map_eq)
+  "asid_pool_at p s \<longleftrightarrow> asid_pools_of False s p \<noteq> None"
+  by (auto simp: obj_at_def in_opt_map_eq obind_def ta_filter_def split:option.splits)
 
 lemma pt_at_eq:
-  "pt_at p s \<longleftrightarrow> pts_of s p \<noteq> None"
-  by (auto simp: obj_at_def in_opt_map_eq)
+  "pt_at p s \<longleftrightarrow> pts_of False s p \<noteq> None"
+  by (auto simp: obj_at_def in_opt_map_eq obind_def ta_filter_def split:option.splits)
 
 lemma valid_asid_tableD:
   "\<lbrakk> riscv_asid_table (arch_state s) x = Some p; valid_asid_table s \<rbrakk> \<Longrightarrow> asid_pool_at p s"
   by (auto simp: valid_asid_table_def asid_pools_at_eq)
 
 lemma dom_asid_pools_of_typ:
-  "dom (asid_pools_of s) = {p. asid_pool_at p s}"
-  by (auto simp: obj_at_def in_opt_map_eq)
+  "dom (asid_pools_of False s) = {p. asid_pool_at p s}"
+  by (auto simp: obj_at_def in_opt_map_eq obind_def ta_filter_def split:option.splits)
 
 lemma dom_asid_pools_of_lift:
   assumes "\<And>T p. f \<lbrace>typ_at (AArch T) p\<rbrace>"
   assumes "\<And>A B. A \<subseteq> B \<Longrightarrow> P A \<Longrightarrow> P B"
-  shows "f \<lbrace>\<lambda>s. P (dom (asid_pools_of s))\<rbrace>"
+  shows "f \<lbrace>\<lambda>s. P (dom (asid_pools_of False s))\<rbrace>"
   by (wpsimp wp: hoare_vcg_set_pred_lift_mono assms simp: dom_asid_pools_of_typ)
 
 lemma aobj_at_default_arch_cap_valid:
@@ -1135,7 +1135,7 @@ lemma state_hyp_refs_of_eqD:
 
 lemma obj_at_state_hyp_refs_ofD:
   "obj_at P p s \<Longrightarrow> \<exists>ko. P ko \<and> state_hyp_refs_of s p = hyp_refs_of ko"
-  by (fastforce simp: obj_at_def state_hyp_refs_of_def f_kheap_def)
+  by (fastforce simp: obj_at_def state_hyp_refs_of_def)
 
 lemma ko_at_state_hyp_refs_ofD:
   "ko_at ko p s \<Longrightarrow> state_hyp_refs_of s p = hyp_refs_of ko"
@@ -1244,7 +1244,7 @@ lemma valid_arch_mdb_eqI:
   by (clarsimp simp: valid_arch_mdb_def)
 
 lemma valid_arch_cap_ref_pspaceI[elim]:
-  "\<lbrakk> valid_arch_cap_ref acap s; f_kheap s = f_kheap s' \<rbrakk> \<Longrightarrow> valid_arch_cap_ref acap s'"
+  "\<lbrakk> valid_arch_cap_ref acap s; kheap s = kheap s' \<rbrakk> \<Longrightarrow> valid_arch_cap_ref acap s'"
   unfolding valid_arch_cap_ref_def
   by (auto intro: obj_at_pspaceI split: arch_cap.split)
 
@@ -1420,7 +1420,7 @@ lemma translate_address_equal_top_slot:
 lemmas min_max_pt_level[simp] = min_absorb2[where x=max_pt_level]
 
 lemma vs_lookup_min_level:
-  "vs_lookup_table bot_level asid vref s = Some (level, p) \<Longrightarrow> bot_level \<le> level"
+  "vs_lookup_table ta_f bot_level asid vref s = Some (level, p) \<Longrightarrow> bot_level \<le> level"
   by (auto simp: vs_lookup_table_def in_omonad not_le split: if_split_asm dest!: pt_walk_min_level)
 
 lemma pt_bits_left_0[simp]:
@@ -1511,12 +1511,12 @@ lemma pt_walk_vref_for_level1:
 
 lemma vs_lookup_vref_for_level1:
   "level \<le> bot_level \<Longrightarrow>
-   vs_lookup_table bot_level asid (vref_for_level vref (level+1)) = vs_lookup_table bot_level asid vref"
+   vs_lookup_table ta_f bot_level asid (vref_for_level vref (level+1)) = vs_lookup_table ta_f bot_level asid vref"
   by (force simp: vs_lookup_table_def pt_walk_vref_for_level1 obind_def split: option.splits)
 
 lemma vs_lookup_vref_for_level:
   "level \<le> bot_level \<Longrightarrow>
-   vs_lookup_table bot_level asid (vref_for_level vref level) = vs_lookup_table bot_level asid vref"
+   vs_lookup_table ta_f bot_level asid (vref_for_level vref level) = vs_lookup_table ta_f bot_level asid vref"
   by (force simp: vs_lookup_table_def pt_walk_vref_for_level obind_def split: option.splits)
 
 lemma riscv_global_pts_global_ref:
@@ -1525,7 +1525,7 @@ lemma riscv_global_pts_global_ref:
 
 lemma valid_global_vspace_mappings_kwD:
   "\<lbrakk> valid_global_vspace_mappings s; vref \<in> kernel_window s \<rbrakk>
-   \<Longrightarrow> translate_address (global_pt s) vref (ptes_of s) = Some (addrFromPPtr vref)"
+   \<Longrightarrow> translate_address (global_pt s) vref (ptes_of False s) = Some (addrFromPPtr vref)"
   by (simp add: valid_global_vspace_mappings_def Let_def)
 
 lemma valid_global_vspace_mappings_aligned[simp]:
@@ -1534,9 +1534,9 @@ lemma valid_global_vspace_mappings_aligned[simp]:
 
 
 lemma vspace_for_asid_SomeD:
-  "vspace_for_asid asid s = Some pt_ptr
+  "vspace_for_asid ta_f asid s = Some pt_ptr
    \<Longrightarrow> \<exists>pool_ptr pool. asid_table s (asid_high_bits_of asid) = Some pool_ptr
-                      \<and> asid_pools_of s pool_ptr = Some pool
+                      \<and> asid_pools_of ta_f s pool_ptr = Some pool
                       \<and> pool (asid_low_bits_of asid) = Some pt_ptr
                       \<and> asid > 0"
   unfolding vspace_for_asid_def
@@ -1544,16 +1544,16 @@ lemma vspace_for_asid_SomeD:
 
 lemma vspace_for_asid_SomeI:
   "\<lbrakk> asid_table s (asid_high_bits_of asid) = Some pool_ptr;
-     asid_pools_of s pool_ptr = Some pool;
+     asid_pools_of ta_f s pool_ptr = Some pool;
      pool (asid_low_bits_of asid) = Some pt_ptr;
      asid > 0 \<rbrakk>
-   \<Longrightarrow> vspace_for_asid asid s = Some pt_ptr"
+   \<Longrightarrow> vspace_for_asid ta_f asid s = Some pt_ptr"
   by (clarsimp simp: vspace_for_asid_def vspace_for_pool_def pool_for_asid_def obind_def)
 
 lemmas ptes_of_def = pte_of_def
 
 lemma ptes_of_pts_of:
-  "ptes_of s pte_ptr = Some pte \<Longrightarrow> pts_of s (pte_ptr && ~~mask pt_bits) \<noteq> None"
+  "ptes_of ta_f s pte_ptr = Some pte \<Longrightarrow> pts_of ta_f s (pte_ptr && ~~mask pt_bits) \<noteq> None"
   by (auto simp: ptes_of_def in_omonad)
 
 lemma ptes_of_eqI:
@@ -1595,8 +1595,8 @@ lemma pt_slot_offset_or_def:
   done
 
 lemma ptes_of_pt_slot_offset:
-  "\<lbrakk> ptes_of s (pt_slot_offset level pt_ptr vref) = Some pte; is_aligned pt_ptr pt_bits \<rbrakk>
-   \<Longrightarrow> pts_of s pt_ptr \<noteq> None"
+  "\<lbrakk> ptes_of ta_f s (pt_slot_offset level pt_ptr vref) = Some pte; is_aligned pt_ptr pt_bits \<rbrakk>
+   \<Longrightarrow> pts_of ta_f s pt_ptr \<noteq> None"
   by (auto dest!: ptes_of_pts_of simp: in_opt_map_eq)
 
 lemma valid_global_vspace_mappings_pt_at:
@@ -1616,12 +1616,12 @@ lemma valid_global_arch_objs_pt_at:
   by fastforce
 
 lemma pool_for_asid_vs_lookup:
-  "(vs_lookup_table asid_pool_level asid vref s = Some (level, p)) =
+  "(vs_lookup_table ta_f asid_pool_level asid vref s = Some (level, p)) =
    (pool_for_asid asid s = Some p \<and> level = asid_pool_level)"
   by (auto simp: vs_lookup_table_def in_omonad)
 
 lemma pool_for_asid_validD:
-  "\<lbrakk> pool_for_asid asid s = Some p; valid_asid_table s \<rbrakk> \<Longrightarrow> asid_pools_of s p \<noteq> None"
+  "\<lbrakk> pool_for_asid asid s = Some p; valid_asid_table s \<rbrakk> \<Longrightarrow> asid_pools_of False s p \<noteq> None"
   by (auto simp: in_opt_map_eq valid_asid_table_def pool_for_asid_def)
 
 lemma constructed_asid_low_bits_of:
@@ -1655,8 +1655,8 @@ lemma pt_walk_level:
   by (fastforce simp: bit0.leq_minus1_less dest: pt_walk_max_level)
 
 lemma vs_lookup_level:
-  "vs_lookup_table bot_level asid vref s = Some (level, p) \<Longrightarrow>
-   vs_lookup_table level asid vref s = Some (level, p)"
+  "vs_lookup_table ta_f bot_level asid vref s = Some (level, p) \<Longrightarrow>
+   vs_lookup_table ta_f level asid vref s = Some (level, p)"
   apply (clarsimp simp: vs_lookup_table_def in_omonad split: if_split_asm)
   apply (erule disjE; clarsimp)
   apply (frule pt_walk_max_level, simp)
@@ -1664,13 +1664,13 @@ lemma vs_lookup_level:
   done
 
 lemma vs_lookup_level_vref1:
-  "vs_lookup_table bot_level asid vref s = Some (level, p)
-   \<Longrightarrow> vs_lookup_table level asid (vref_for_level vref (level+1)) s = Some (level, p)"
+  "vs_lookup_table ta_f bot_level asid vref s = Some (level, p)
+   \<Longrightarrow> vs_lookup_table ta_f level asid (vref_for_level vref (level+1)) s = Some (level, p)"
   by (simp add: vs_lookup_level vs_lookup_vref_for_level1)
 
 lemma vs_lookup_level_vref:
-  "vs_lookup_table bot_level asid vref s = Some (level, p)
-   \<Longrightarrow> vs_lookup_table level asid (vref_for_level vref level) s = Some (level, p)"
+  "vs_lookup_table ta_f bot_level asid vref s = Some (level, p)
+   \<Longrightarrow> vs_lookup_table ta_f level asid (vref_for_level vref level) s = Some (level, p)"
   by (simp add: vs_lookup_level vs_lookup_vref_for_level)
 
 lemma pt_walk_same[simp]:
@@ -1678,34 +1678,34 @@ lemma pt_walk_same[simp]:
   by (auto simp: pt_walk.simps)
 
 lemma vs_lookup_asid_pool:
-  "\<lbrakk> vs_lookup_table bot_level asid vref s = Some (asid_pool_level, p); valid_asid_table s \<rbrakk>
-  \<Longrightarrow> asid_pools_of s p \<noteq> None"
+  "\<lbrakk> vs_lookup_table False bot_level asid vref s = Some (asid_pool_level, p); valid_asid_table s \<rbrakk>
+  \<Longrightarrow> asid_pools_of False s p \<noteq> None"
   by (drule vs_lookup_level)
      (auto dest!: pool_for_asid_validD simp: pool_for_asid_vs_lookup)
 
 lemma pt_lookup_vs_lookup_eq:
   "\<lbrakk> bot_level \<le> max_pt_level; 0 < asid \<rbrakk> \<Longrightarrow>
-   vs_lookup_table bot_level asid vref = do {
-      pt \<leftarrow> vspace_for_asid asid;
-      pt_walk max_pt_level bot_level pt vref \<circ> ptes_of
+   vs_lookup_table ta_f bot_level asid vref = do {
+      pt \<leftarrow> vspace_for_asid ta_f asid;
+      pt_walk max_pt_level bot_level pt vref \<circ> ptes_of ta_f
   }"
   by (auto simp: vs_lookup_table_def vspace_for_asid_def obind_assoc intro!: opt_bind_cong)
 
 lemma vspace_for_asid_0:
-  "vspace_for_asid asid s = Some pt \<Longrightarrow> 0 < asid"
+  "vspace_for_asid ta_f asid s = Some pt \<Longrightarrow> 0 < asid"
   by (simp add: vspace_for_asid_def in_omonad split: if_split_asm)
 
 lemma pt_lookup_vs_lookupI:
-  "\<lbrakk> vspace_for_asid asid s = Some pt;
-     pt_walk max_pt_level bot_level pt vref (ptes_of s) = Some (level, p);
+  "\<lbrakk> vspace_for_asid ta_f asid s = Some pt;
+     pt_walk max_pt_level bot_level pt vref (ptes_of ta_f s) = Some (level, p);
      bot_level \<le> max_pt_level \<rbrakk> \<Longrightarrow>
-   vs_lookup_table bot_level asid vref s = Some (level, p)"
+   vs_lookup_table ta_f bot_level asid vref s = Some (level, p)"
   by (frule vspace_for_asid_0) (auto simp: pt_lookup_vs_lookup_eq obind_def)
 
 lemma pt_lookup_slot_vs_lookup_slotI:
-  "\<lbrakk> vspace_for_asid asid s = Some pt_ptr;
-     pt_lookup_slot pt_ptr vref (ptes_of s) = Some (level, slot) \<rbrakk>
-   \<Longrightarrow> vs_lookup_slot level asid vref s = Some (level, slot) \<and> level \<le> max_pt_level"
+  "\<lbrakk> vspace_for_asid ta_f asid s = Some pt_ptr;
+     pt_lookup_slot pt_ptr vref (ptes_of ta_f s) = Some (level, slot) \<rbrakk>
+   \<Longrightarrow> vs_lookup_slot ta_f level asid vref s = Some (level, slot) \<and> level \<le> max_pt_level"
   unfolding pt_lookup_slot_def pt_lookup_slot_from_level_def vs_lookup_slot_def
   apply (clarsimp simp: in_omonad)
   apply (drule (1) pt_lookup_vs_lookupI, simp)
@@ -1714,28 +1714,28 @@ lemma pt_lookup_slot_vs_lookup_slotI:
   done
 
 lemma vspace_for_asid_vs_lookup:
-  "vspace_for_asid asid s = Some pt \<Longrightarrow>
-   vs_lookup_table max_pt_level asid 0 s = Some (max_pt_level, pt)"
+  "vspace_for_asid ta_f asid s = Some pt \<Longrightarrow>
+   vs_lookup_table ta_f max_pt_level asid 0 s = Some (max_pt_level, pt)"
   by (clarsimp simp: vspace_for_asid_def vs_lookup_table_def in_omonad pt_walk.simps)
 
 lemma ptes_of_ptsD:
-  assumes p: "ptes_of s pte_ptr = Some pte"
+  assumes p: "ptes_of ta_f s pte_ptr = Some pte"
   assumes a: "is_aligned pte_ptr table_size"
-  shows "pts_of s pte_ptr \<noteq> None"
+  shows "pts_of ta_f s pte_ptr \<noteq> None"
 proof -
   from a have "pte_ptr && ~~mask pt_bits = pte_ptr" by (simp add: pt_bits_def)
   with p show ?thesis by (auto dest!: ptes_of_pts_of)
 qed
 
 lemma pte_at_eq:
-  "pte_at p s = (ptes_of s p \<noteq> None)"
-  by (auto simp: obj_at_def pte_at_def in_omonad pte_of_def)
+  "pte_at p s = (ptes_of False s p \<noteq> None)"
+  by (auto simp: obj_at_def pte_at_def in_omonad pte_of_def ta_filter_def)
 
 lemma valid_vspace_objsI [intro?]:
   "(\<And>p ao asid vref level.
-       \<lbrakk> vs_lookup_table level asid (vref_for_level vref (level+1)) s = Some (level, p);
+       \<lbrakk> vs_lookup_table False level asid (vref_for_level vref (level+1)) s = Some (level, p);
          vref \<in> user_region;
-         aobjs_of s p = Some ao \<rbrakk>
+         aobjs_of False s p = Some ao \<rbrakk>
        \<Longrightarrow> valid_vspace_obj level ao s)
   \<Longrightarrow> valid_vspace_objs s"
   by (fastforce simp: valid_vspace_objs_def dest: vs_lookup_level_vref1)
@@ -1755,20 +1755,22 @@ lemma ptpte_level_0_valid_pte:
 lemma pool_for_asid_valid_vspace_objs:
   "\<lbrakk> pool_for_asid asid s = Some p;
      valid_vspace_objs s; valid_asid_table s \<rbrakk>
-   \<Longrightarrow> \<exists>pool. asid_pools_of s p = Some pool \<and> valid_vspace_obj asid_pool_level (ASIDPool pool) s"
+   \<Longrightarrow> \<exists>pool. asid_pools_of False s p = Some pool \<and> valid_vspace_obj asid_pool_level (ASIDPool pool) s"
   unfolding valid_vspace_objs_def
   by (fastforce intro: pool_for_asid_vs_lookup[THEN iffD2]
                  dest: pool_for_asid_validD
                  simp: in_opt_map_eq)
 
 lemma vspace_for_asid_valid_pt:
-  "\<lbrakk> vspace_for_asid asid s = Some root_pt;
+  "\<lbrakk> vspace_for_asid False asid s = Some root_pt;
      valid_vspace_objs s; valid_asid_table s \<rbrakk>
-   \<Longrightarrow> \<exists>pt. pts_of s root_pt = Some pt \<and> valid_vspace_obj max_pt_level (PageTable pt) s"
+   \<Longrightarrow> \<exists>pt. pts_of False s root_pt = Some pt \<and> valid_vspace_obj max_pt_level (PageTable pt) s"
   apply (frule vspace_for_asid_vs_lookup)
   apply (clarsimp simp: vspace_for_asid_def)
   apply (frule (2) pool_for_asid_valid_vspace_objs)
+  sorry (* Broken by timeprot-use-f-kheap. -robs
   by (fastforce simp: in_opt_map_eq valid_vspace_objs_def pt_at_eq vspace_for_pool_def)
+*)
 
 lemma pt_slot_offset_vref:
   "\<lbrakk> level < level'; is_aligned vref (pt_bits_left level') \<rbrakk> \<Longrightarrow>
@@ -1785,36 +1787,38 @@ lemma pt_slot_offset_vref_for_level_eq:
   by (simp add: vref_for_level_def pt_slot_offset_vref)
 
 lemma vspace_for_pool_None_upd_idem:
-  "vspace_for_pool pool_ptr asid ((asid_pools_of s)(p := None)) = Some table_ptr
-   \<Longrightarrow> vspace_for_pool pool_ptr asid (asid_pools_of s) = Some table_ptr"
+  "vspace_for_pool pool_ptr asid ((asid_pools_of ta_f s)(p := None)) = Some table_ptr
+   \<Longrightarrow> vspace_for_pool pool_ptr asid (asid_pools_of ta_f s) = Some table_ptr"
   by (clarsimp simp: vspace_for_pool_def obind_def split: option.splits if_splits)
 
 lemma vs_lookup_max_pt_levelD:
-  "vs_lookup_table max_pt_level asid vref s = Some (max_pt_level, root_pt)
+  "vs_lookup_table ta_f max_pt_level asid vref s = Some (max_pt_level, root_pt)
    \<Longrightarrow> \<exists>pool_ptr. pool_for_asid asid s = Some pool_ptr \<and>
-                  vspace_for_pool pool_ptr asid (asid_pools_of s) = Some root_pt"
+                  vspace_for_pool pool_ptr asid (asid_pools_of ta_f s) = Some root_pt"
   by (clarsimp simp: vs_lookup_table_def)
 
 lemma vs_lookup_max_pt_levelI:
   "\<lbrakk> pool_for_asid asid s = Some pool_ptr;
-     vspace_for_pool pool_ptr asid (asid_pools_of s) = Some root_pt \<rbrakk>
-   \<Longrightarrow> vs_lookup_table max_pt_level asid vref s = Some (max_pt_level, root_pt)"
+     vspace_for_pool pool_ptr asid (asid_pools_of ta_f s) = Some root_pt \<rbrakk>
+   \<Longrightarrow> vs_lookup_table ta_f max_pt_level asid vref s = Some (max_pt_level, root_pt)"
   by (clarsimp simp: vs_lookup_table_def in_omonad)
 
 lemma vs_lookup_table_max_pt_level_SomeD:
-  "\<lbrakk> vs_lookup_table max_pt_level asid vref s = Some (level, p) \<rbrakk>
-   \<Longrightarrow> \<exists>pool. pool_for_asid asid s = Some pool \<and> vspace_for_pool pool asid (asid_pools_of s) = Some p"
+  "\<lbrakk> vs_lookup_table ta_f max_pt_level asid vref s = Some (level, p) \<rbrakk>
+   \<Longrightarrow> \<exists>pool. pool_for_asid asid s = Some pool \<and> vspace_for_pool pool asid (asid_pools_of ta_f s) = Some p"
   by (clarsimp simp: vs_lookup_table_def in_omonad)
 
 lemma vs_lookup_max_pt_valid:
-  "\<lbrakk> vs_lookup_table max_pt_level asid vref s = Some (max_pt_level, root_pt);
+  "\<lbrakk> vs_lookup_table False max_pt_level asid vref s = Some (max_pt_level, root_pt);
      vref \<in> user_region;
      valid_vspace_objs s; valid_asid_table s \<rbrakk>
-   \<Longrightarrow> \<exists>pt. pts_of s root_pt = Some pt \<and> valid_vspace_obj max_pt_level (PageTable pt) s"
+   \<Longrightarrow> \<exists>pt. pts_of False s root_pt = Some pt \<and> valid_vspace_obj max_pt_level (PageTable pt) s"
   apply (frule vs_lookup_max_pt_levelD)
   apply clarsimp
   apply (frule (2) pool_for_asid_valid_vspace_objs)
+  sorry (* Broken by timeprot-use-f-kheap. -robs
   by (fastforce simp: in_opt_map_eq valid_vspace_objs_def pt_at_eq vspace_for_pool_def)
+*)
 
 lemma aligned_vref_for_level_eq:
   "is_aligned vref (pt_bits_left level) = (vref_for_level vref level = vref)"
@@ -1872,8 +1876,8 @@ lemma table_index_offset_pt_bits_left:
                 ptTranslationBits_def ucast_ucast_mask[where 'a=9, simplified, symmetric])
 
 lemma vs_lookup_slot_level:
-  "vs_lookup_slot bot_level asid vref s = Some (level, p) \<Longrightarrow>
-   vs_lookup_slot level asid vref s = Some (level, p)"
+  "vs_lookup_slot ta_f bot_level asid vref s = Some (level, p) \<Longrightarrow>
+   vs_lookup_slot ta_f level asid vref s = Some (level, p)"
   apply (clarsimp simp: vs_lookup_slot_def in_omonad)
   apply (drule vs_lookup_level)
   apply (force split: if_splits)
@@ -1889,7 +1893,7 @@ lemma vs_lookup_target_level:
 
 lemma vs_lookup_slot_vref_for_level:
   "level \<le> bot_level \<Longrightarrow>
-   vs_lookup_slot bot_level asid (vref_for_level vref level) = vs_lookup_slot bot_level asid vref"
+   vs_lookup_slot ta_f bot_level asid (vref_for_level vref level) = vs_lookup_slot ta_f bot_level asid vref"
   apply (simp add: vs_lookup_slot_def vs_lookup_vref_for_level)
   apply (rule ext, rule obind_eqI, rule refl)
   apply (clarsimp dest!: vs_lookup_min_level)
@@ -1901,12 +1905,12 @@ lemma vs_lookup_target_vref_for_level:
   by (simp add: vs_lookup_target_def vs_lookup_slot_vref_for_level)
 
 lemma pts_of_ko_at:
-  "(pts_of s p = Some pt) = ako_at (PageTable pt) p s"
-  by (simp add: obj_at_def in_opt_map_eq)
+  "(pts_of False s p = Some pt) = ako_at (PageTable pt) p s"
+  by (simp add: obj_at_def in_opt_map_eq obind_def ta_filter_def split:option.splits)
 
 lemma asid_pools_of_ko_at:
-  "(asid_pools_of s p = Some ap) = ako_at (ASIDPool ap) p s"
-  by (simp add: obj_at_def in_opt_map_eq)
+  "(asid_pools_of False s p = Some ap) = ako_at (ASIDPool ap) p s"
+  by (simp add: obj_at_def in_opt_map_eq obind_def ta_filter_def split:option.splits)
 
 lemma a_type_ArchObj[simp]:
   "a_type (ArchObj ao) = AArch (aa_type ao)"
@@ -1914,7 +1918,7 @@ lemma a_type_ArchObj[simp]:
 
 lemma typ_at_aobjs:
   "typ_at (AArch T) p s = (atyps_of s p = Some T)"
-  by (auto simp: obj_at_def in_opt_map_eq)
+  by (auto simp: obj_at_def in_opt_map_eq obind_def ta_filter_def split:option.splits)
 
 lemma geq_max_pt_level:
   "(max_pt_level \<le> level) = (level = max_pt_level \<or> level = asid_pool_level)"
@@ -1922,12 +1926,12 @@ lemma geq_max_pt_level:
 
 lemma vs_lookup_asid_pool_level_eq:
   "asid_table s' = asid_table s \<Longrightarrow>
-   vs_lookup_table asid_pool_level asid vref s' = vs_lookup_table asid_pool_level asid vref s"
+   vs_lookup_table ta_f asid_pool_level asid vref s' = vs_lookup_table ta_f asid_pool_level asid vref s"
   by (simp add: vs_lookup_table_def obind_def pool_for_asid_def split: option.splits)
 
 lemma vs_lookup_max_pt_level_eq:
-  "\<lbrakk> asid_table s' = asid_table s; asid_pools_of s' = asid_pools_of s \<rbrakk> \<Longrightarrow>
-   vs_lookup_table max_pt_level asid vref s' = vs_lookup_table max_pt_level asid vref s"
+  "\<lbrakk> asid_table s' = asid_table s; asid_pools_of ta_f s' = asid_pools_of ta_f s \<rbrakk> \<Longrightarrow>
+   vs_lookup_table ta_f max_pt_level asid vref s' = vs_lookup_table ta_f max_pt_level asid vref s"
   by (clarsimp simp: vs_lookup_table_def obind_def pool_for_asid_def vspace_for_pool_def pt_walk.simps
               split: option.splits)
 
@@ -1988,21 +1992,21 @@ lemma pt_walk_split_Some:
 
 lemma vs_lookup_split_max_pt_level:
   "level \<le> max_pt_level \<Longrightarrow>
-   vs_lookup_table level asid vref = do {
-     (level',pt) \<leftarrow> vs_lookup_table max_pt_level asid vref;
+   vs_lookup_table ta_f level asid vref = do {
+     (level',pt) \<leftarrow> vs_lookup_table ta_f  max_pt_level asid vref;
      if level' = max_pt_level
-     then pt_walk max_pt_level level pt vref \<circ> ptes_of
+     then pt_walk max_pt_level level pt vref \<circ> ptes_of ta_f
      else oreturn (level', pt)
    }"
   by (auto simp: vs_lookup_table_def obind_assoc intro!: opt_bind_cong opt_bind_cong_apply)
 
 lemma vs_lookup_split:
   "\<lbrakk> level \<le> level'; level' \<le> max_pt_level \<rbrakk> \<Longrightarrow>
-   vs_lookup_table level asid vref =
+   vs_lookup_table ta_f level asid vref =
    do {
-      (level'', pt) \<leftarrow> vs_lookup_table level' asid vref;
+      (level'', pt) \<leftarrow> vs_lookup_table ta_f level' asid vref;
       if level'' = level'
-      then pt_walk level' level pt vref \<circ> ptes_of
+      then pt_walk level' level pt vref \<circ> ptes_of ta_f
       else oreturn (level'', pt)
     }"
   apply (cases "level' < max_pt_level")
@@ -2022,9 +2026,9 @@ lemma vs_lookup_split:
   done
 
 lemma vs_lookup_table_split_last_Some:
-  "\<lbrakk> vs_lookup_table level asid vref s = Some (level, p); level < max_pt_level \<rbrakk>
-   \<Longrightarrow> \<exists>p' pte. vs_lookup_table (level+1) asid vref s = Some (level+1, p')
-            \<and> ptes_of s (pt_slot_offset (level + 1) p' vref) = Some pte \<and> p = pptr_from_pte pte
+  "\<lbrakk> vs_lookup_table ta_f level asid vref s = Some (level, p); level < max_pt_level \<rbrakk>
+   \<Longrightarrow> \<exists>p' pte. vs_lookup_table ta_f (level+1) asid vref s = Some (level+1, p')
+            \<and> ptes_of ta_f s (pt_slot_offset (level + 1) p' vref) = Some pte \<and> p = pptr_from_pte pte
             \<and> is_PageTablePTE pte"
   apply (clarsimp simp: vs_lookup_table_def in_omonad asid_pool_level_eq
                          vm_level_less_max_pt_level)
@@ -2036,16 +2040,16 @@ lemma vs_lookup_table_split_last_Some:
 
 lemma vs_lookup_split_max_pt_level_Some:
   "level \<le> max_pt_level \<Longrightarrow>
-   (vs_lookup_table level asid vref s = Some (level, p)) =
-   (\<exists>pt. vs_lookup_table max_pt_level asid vref s = Some (max_pt_level, pt)
-         \<and> pt_walk max_pt_level level pt vref (ptes_of s) = Some (level, p))"
+   (vs_lookup_table ta_f level asid vref s = Some (level, p)) =
+   (\<exists>pt. vs_lookup_table ta_f max_pt_level asid vref s = Some (max_pt_level, pt)
+         \<and> pt_walk max_pt_level level pt vref (ptes_of ta_f s) = Some (level, p))"
   by (auto simp: vs_lookup_table_def in_omonad not_le split: if_split_asm)
 
 lemma vs_lookup_split_Some:
   "\<lbrakk> level \<le> level'; level' \<le> max_pt_level \<rbrakk> \<Longrightarrow>
-   (vs_lookup_table level asid vref s = Some (level, p)) =
-   (\<exists>pt. vs_lookup_table level' asid vref s = Some (level', pt)
-         \<and> pt_walk level' level pt vref (ptes_of s) = Some (level, p))"
+   (vs_lookup_table ta_f level asid vref s = Some (level, p)) =
+   (\<exists>pt. vs_lookup_table ta_f level' asid vref s = Some (level', pt)
+         \<and> pt_walk level' level pt vref (ptes_of ta_f s) = Some (level, p))"
   apply (cases "level' < max_pt_level")
    apply (subst vs_lookup_split_max_pt_level_Some, simp)
    apply (subst (2) vs_lookup_split_max_pt_level_Some, simp)
@@ -2059,8 +2063,8 @@ lemmas vs_lookup_splitD = vs_lookup_split_Some[rotated, THEN iffD1, rotated -1]
 
 lemma valid_vspace_objsD:
   "\<lbrakk> valid_vspace_objs s;
-     vs_lookup_table bot_level asid vref s = Some (level, p);
-     vref \<in> user_region; aobjs_of s p = Some ao \<rbrakk> \<Longrightarrow>
+     vs_lookup_table False bot_level asid vref s = Some (level, p);
+     vref \<in> user_region; aobjs_of False s p = Some ao \<rbrakk> \<Longrightarrow>
    valid_vspace_obj level ao s"
   by (simp add: valid_vspace_objs_def)
 
@@ -2182,8 +2186,8 @@ lemma ptr_from_pte_aligned[simp,intro!]:
   by (auto simp: addr_from_ppn_def is_aligned_shift)
 
 lemma pspace_aligned_pts_ofD:
-  "\<lbrakk> pspace_aligned s; pts_of s pt_ptr \<noteq> None \<rbrakk> \<Longrightarrow> is_aligned pt_ptr pt_bits"
-  by (fastforce dest: pspace_alignedD simp: in_omonad bit_simps f_kheap_def split: if_splits)
+  "\<lbrakk> pspace_aligned s; pts_of False s pt_ptr \<noteq> None \<rbrakk> \<Longrightarrow> is_aligned pt_ptr pt_bits"
+  by (fastforce dest: pspace_alignedD simp: in_omonad bit_simps ta_filter_def)
 
 lemma user_region_slots:
   "vref \<in> user_region \<Longrightarrow> ucast (pt_index max_pt_level vref) \<notin> kernel_mapping_slots"
@@ -2194,11 +2198,11 @@ lemma user_region_slots:
 
 lemma valid_vspace_objs_strongD:
   "\<lbrakk> valid_vspace_objs s;
-     vs_lookup_table bot_level asid vref s = Some (level, pt_ptr);
+     vs_lookup_table False bot_level asid vref s = Some (level, pt_ptr);
      vref \<in> user_region;
      level \<le> max_pt_level;
      valid_asid_table s; pspace_aligned s \<rbrakk> \<Longrightarrow>
-   \<exists>pt. pts_of s pt_ptr = Some pt \<and> valid_vspace_obj level (PageTable pt) s"
+   \<exists>pt. pts_of False s pt_ptr = Some pt \<and> valid_vspace_obj level (PageTable pt) s"
   supply valid_vspace_obj.simps[simp del]
   apply (drule vs_lookup_level)
   apply (induct level arbitrary: pt_ptr rule: bit0.from_top_induct[where y="max_pt_level"])
@@ -2211,7 +2215,7 @@ lemma valid_vspace_objs_strongD:
   apply (drule_tac x=pt in meta_spec)
   apply clarsimp
   apply (subst (asm) pt_walk.simps)
-  apply (clarsimp simp: in_omonad f_kheap_def split: if_split_asm)
+  apply (clarsimp simp: in_omonad split: if_split_asm)
   apply (subst (asm) valid_vspace_obj.simps)
   apply (frule (1) pspace_alignedD)
   apply (clarsimp simp: ptes_of_def in_omonad pt_slot_offset_offset
@@ -2220,10 +2224,12 @@ lemma valid_vspace_objs_strongD:
    apply (clarsimp simp: user_region_slots)
   apply (clarsimp simp: is_PageTablePTE_def pptr_from_pte_def pt_at_eq in_omonad)
   apply (drule (2) valid_vspace_objsD)
-   apply (simp add: in_omonad)
-  apply(clarsimp simp:f_kheap_def split:if_splits)
-  apply blast
+   apply (clarsimp simp: in_omonad ta_filter_def obind_def split:if_splits option.splits)
+   apply(rule conjI)
+    sorry (* Broken by timeprot-use-f-kheap. -robs
   done
+*)
+. (* DOWN TO HERE. -robs
 
 lemma pt_walk_is_aligned:
   "\<lbrakk> pt_walk level bot_level p vref' ptes = Some (level', p');
